lib: apply consistent style to OptionMonad
Signed-off-by: Gerwin Klein <gerwin.klein@proofcraft.systems>

lib/Monads/OptionMonad.thy
@@ -18,19 +18,29 @@ theory OptionMonad (* FIXME: this is really a Reader_Option_Monad *)
     Less_Monad_Syntax
 begin
 
+section \<open>Projections\<close>
+
 type_synonym ('s,'a) lookup = "'s \<Rightarrow> 'a option"
 
 text \<open>Similar to map_option but the second function returns option as well\<close>
-definition
-  opt_map :: "('s,'a) lookup \<Rightarrow> ('a \<Rightarrow> 'b option) \<Rightarrow> ('s,'b) lookup" (infixl "|>" 54)
-where
+definition opt_map :: "('s,'a) lookup \<Rightarrow> ('a \<Rightarrow> 'b option) \<Rightarrow> ('s,'b) lookup" (infixl "|>" 54) where
   "f |> g \<equiv> \<lambda>s. case f s of None \<Rightarrow> None | Some x \<Rightarrow> g x"
 
 abbreviation opt_map_Some :: "('s \<rightharpoonup> 'a) \<Rightarrow> ('a \<Rightarrow> 'b) \<Rightarrow> 's \<rightharpoonup> 'b" (infixl "||>" 54) where
   "f ||> g \<equiv> f |> (Some \<circ> g)"
+
 lemmas opt_map_Some_def = opt_map_def
 
-lemma opt_map_cong [fundef_cong]:
+definition map_set :: "('a \<Rightarrow> 'b set option) \<Rightarrow> 'a \<Rightarrow> 'b set" where
+  "map_set f \<equiv> case_option {} id \<circ> f"
+
+definition opt_pred :: "('a \<Rightarrow> bool) \<Rightarrow> ('b \<Rightarrow> 'a option) \<Rightarrow> ('b \<Rightarrow> bool)" (infixl "|<" 55) where
+  "P |< proj \<equiv> (\<lambda>x. case_option False P (proj x))"
+
+
+subsection \<open>Lemmas for @{const opt_map}\<close>
+
+lemma opt_map_cong[fundef_cong]:
   "\<lbrakk> f = f'; \<And>v s. f s = Some v \<Longrightarrow> g v = g' v\<rbrakk> \<Longrightarrow> f |> g = f' |> g'"
   by (rule ext) (simp add: opt_map_def split: option.splits)
 
@@ -78,8 +88,7 @@ lemma opt_map_Some_upd_Some:
   "f(x \<mapsto> v) ||> g = (f ||> g)(x \<mapsto> g v)"
   by (simp add: opt_map_upd_Some)
 
-lemmas opt_map_upd[simp]
-  = opt_map_upd_None opt_map_upd_Some opt_map_Some_upd_Some
+lemmas opt_map_upd[simp] = opt_map_upd_None opt_map_upd_Some opt_map_Some_upd_Some
 
 lemma opt_map_upd_triv:
   "t k = Some x \<Longrightarrow> (t |> f)(k := f x) = t |> f"
@@ -96,17 +105,16 @@ lemma opt_map_upd_triv_None:
 lemmas opt_map_upd_triv_simps = opt_map_upd_triv opt_map_Some_upd_triv opt_map_upd_triv_None
 
 lemma opt_map_foldr_upd:
-  "(foldr (\<lambda>p kh. kh(p := new)) ptrs f)|> g
+  "foldr (\<lambda>p kh. kh(p := new)) ptrs f |> g
    = foldr (\<lambda>p kh. kh(p := (case new of Some x \<Rightarrow> g x | _ \<Rightarrow> None))) ptrs (f |> g)"
   by (induct ptrs arbitrary: new; clarsimp split: option.splits)
 
 lemma opt_map_Some_foldr_upd:
-  "(foldr (\<lambda>p kh. kh(p := new)) ptrs f) ||> g
-   = foldr (\<lambda>p kh. kh(p := (case new of Some x \<Rightarrow> Some (g x) | _ \<Rightarrow>  None))) ptrs (f ||> g)"
-  by (induct ptrs arbitrary: new; clarsimp split: option.splits)
+  "foldr (\<lambda>p kh. kh(p := new)) ptrs f ||> g
+   = foldr (\<lambda>p kh. kh(p := map_option g new)) ptrs (f ||> g)"
+  by (induct ptrs arbitrary: new; clarsimp simp: map_option_case split: option.splits)
 
-lemmas opt_map_foldr_upd_simps
-  = opt_map_foldr_upd opt_map_Some_foldr_upd
+lemmas opt_map_foldr_upd_simps = opt_map_foldr_upd opt_map_Some_foldr_upd
 
 lemma opt_map_Some_comp[simp]:
   "f ||> g ||> h = f ||> h o g"
@@ -138,8 +146,7 @@ lemma opt_map_Some_eta_fold:
   by (simp add: o_def)
 
 lemma case_opt_map_distrib:
-  "((\<lambda>s. case_option None g (f s)) |> h)
-   = ((\<lambda>s. case_option None (g |> h) (f s)))"
+  "(\<lambda>s. case_option None g (f s)) |> h = (\<lambda>s. case_option None (g |> h) (f s))"
   by (fastforce simp: opt_map_def split: option.splits)
 
 lemma opt_map_apply_left_eq:
@@ -152,20 +159,14 @@ declare None_upd_eq[simp]
 lemma "\<lbrakk> (f |> g) x = None; g v = None \<rbrakk> \<Longrightarrow> f(x \<mapsto> v) |> g = f |> g"
   by simp
 
-definition map_set :: "('a \<Rightarrow> 'b set option) \<Rightarrow> 'a \<Rightarrow> 'b set" where
-  "map_set f \<equiv> case_option {} id \<circ> f"
-
-(* opt_pred *)
-
-definition opt_pred :: "('a \<Rightarrow> bool) \<Rightarrow> ('b \<Rightarrow> 'a option) \<Rightarrow> ('b \<Rightarrow> bool)" (infixl "|<" 55) where
-  "P |< proj \<equiv> (\<lambda>x. case_option False P (proj x))"
+subsection \<open>Lemmas for @{const opt_pred}\<close>
 
 lemma opt_pred_conj:
-  "((P1 |< hp) p \<and> (P2 |< hp) p) = (((P1 and P2) |< hp) p)"
+  "((P |< hp) p \<and> (Q |< hp) p) = ((P and Q) |< hp) p"
   by (fastforce simp: pred_conj_def opt_pred_def split: option.splits)
 
 lemma opt_pred_disj:
-  "((P1 |< hp) p \<or> (P2 |< hp) p) = (((P1 or P2) |< hp) p)"
+  "((P |< hp) p \<or> (Q |< hp) p) = ((P or Q) |< hp) p"
   by (fastforce simp: pred_disj_def opt_pred_def split: option.splits)
 
 lemma in_opt_pred:
@@ -179,40 +180,38 @@ lemma opt_predE:
   by (blast dest: opt_predD)
 
 lemma opt_pred_unfold_map:
-  "(P |< (f |> g)) = ((P |< g) |< f)"
+  "P |< (f |> g) = P |< g |< f"
   by (fastforce simp: opt_map_def in_opt_pred split: option.splits)
 
 lemma opt_pred_unfold_proj:
-  "(P |< (f ||> g))=  (P o g |< f)"
+  "P |< (f ||> g) = P o g |< f"
   by (clarsimp simp: opt_map_def opt_pred_def split: option.splits)
 
-(* This rule is useful when fun_upd_apply is not in the simp set: *)
 lemma opt_pred_proj_upd_eq[simp]:
   "(P |< proj (p \<mapsto> v)) p = P v"
   by (simp add: in_opt_pred)
 
 
-(* obind, etc. *)
+section \<open>The Reader Option Monad\<close>
 
-definition
-  obind :: "('s,'a) lookup \<Rightarrow> ('a \<Rightarrow> ('s,'b) lookup) \<Rightarrow> ('s,'b) lookup" (infixl "|>>" 53)
-where
+definition obind :: "('s,'a) lookup \<Rightarrow> ('a \<Rightarrow> ('s,'b) lookup) \<Rightarrow> ('s,'b) lookup" (infixl "|>>" 53)
+  where
   "f |>> g \<equiv> \<lambda>s. case f s of None \<Rightarrow> None | Some x \<Rightarrow> g x s"
 
 (* Enable "do { .. }" syntax *)
 adhoc_overloading
   Monad_Syntax.bind obind
 
-definition
+definition ofail :: "('s, 'a) lookup" where
   "ofail = K None"
 
-definition
+definition oreturn :: "'a \<Rightarrow> ('s, 'a) lookup" where
   "oreturn = K o Some"
 
-definition
+definition oassert :: "bool \<Rightarrow> ('s, unit) lookup" where
   "oassert P \<equiv> if P then oreturn () else ofail"
 
-definition
+definition oassert_opt :: "'a option \<Rightarrow> ('s, 'a) lookup" where
   "oassert_opt r \<equiv> case r of None \<Rightarrow> ofail | Some x \<Rightarrow> oreturn x"
 
 definition oapply :: "'a \<Rightarrow> ('a \<Rightarrow> 'b option) \<Rightarrow> 'b option" where
@@ -231,19 +230,18 @@ definition owhen :: "bool \<Rightarrow> ('s, unit) lookup \<Rightarrow> ('s, uni
   "owhen P f \<equiv> if P then f else oreturn ()"
 
 (* Reader monad interface: *)
-abbreviation (input)
+abbreviation (input) ask :: "('s, 's) lookup" where
   "ask \<equiv> Some"
 
-definition
+definition asks :: "('s \<Rightarrow> 'a) \<Rightarrow> ('s, 'a) lookup" where
   "asks f = do { v <- ask; oreturn (f v) }"
 
-abbreviation
+abbreviation ogets :: "('s \<Rightarrow> 'a) \<Rightarrow> ('s, 'a) lookup" where
   "ogets \<equiv> asks"
 
 text \<open>
-  If the result can be an exception.
-  Corresponding bindE would be analogous to lifting in NonDetMonad.
-\<close>
+  Integration with exception monad.
+  Corresponding bindE would be analogous to lifting in NonDetMonad.\<close>
 
 definition
   "oreturnOk x = K (Some (Inr x))"
@@ -260,11 +258,15 @@ definition
 definition
   "oskip \<equiv> oreturn ()"
 
-text \<open>Monad laws\<close>
-lemma oreturn_bind [simp]: "(oreturn x |>> f) = f x"
+
+subsection \<open>Monad laws\<close>
+
+lemma oreturn_bind[simp]:
+  "(oreturn x |>> f) = f x"
   by (auto simp add: oreturn_def obind_def K_def)
 
-lemma obind_return [simp]: "(m |>> oreturn) = m"
+lemma obind_return[simp]:
+  "(m |>> oreturn) = m"
   by (auto simp add: oreturn_def obind_def K_def split: option.splits)
 
 lemma obind_assoc:
@@ -272,7 +274,7 @@ lemma obind_assoc:
   by (auto simp add: oreturn_def obind_def K_def split: option.splits)
 
 
-text \<open>Binding fail\<close>
+subsection \<open>Binding and fail\<close>
 
 lemma obind_fail [simp]:
   "f |>> (\<lambda>_. ofail) = ofail"
@@ -283,53 +285,53 @@ lemma ofail_bind [simp]:
   by (auto simp add: ofail_def obind_def K_def split: option.splits)
 
 
+subsection \<open>Function package setup\<close>
 
-text \<open>Function package setup\<close>
-lemma opt_bind_cong [fundef_cong]:
+lemma opt_bind_cong[fundef_cong]:
   "\<lbrakk> f = f'; \<And>v s. f' s = Some v \<Longrightarrow> g v s = g' v s \<rbrakk> \<Longrightarrow> f |>> g = f' |>> g'"
   by (rule ext) (simp add: obind_def split: option.splits)
 
-lemma opt_bind_cong_apply [fundef_cong]:
+lemma opt_bind_cong_apply[fundef_cong]:
   "\<lbrakk> f s = f' s; \<And>v. f' s = Some v \<Longrightarrow> g v s = g' v s \<rbrakk> \<Longrightarrow> (f |>> g) s = (f' |>> g') s"
   by (simp add: obind_def split: option.splits)
 
-lemma oassert_bind_cong [fundef_cong]:
+lemma oassert_bind_cong[fundef_cong]:
   "\<lbrakk> P = P'; P' \<Longrightarrow> m = m' \<rbrakk> \<Longrightarrow> oassert P |>> m = oassert P' |>> m'"
   by (auto simp: oassert_def)
 
-lemma oassert_bind_cong_apply [fundef_cong]:
+lemma oassert_bind_cong_apply[fundef_cong]:
   "\<lbrakk> P = P'; P' \<Longrightarrow> m () s = m' () s \<rbrakk> \<Longrightarrow> (oassert P |>> m) s = (oassert P' |>> m') s"
   by (auto simp: oassert_def)
 
-lemma oreturn_bind_cong [fundef_cong]:
+lemma oreturn_bind_cong[fundef_cong]:
   "\<lbrakk> x = x'; m x' = m' x' \<rbrakk> \<Longrightarrow> oreturn x |>> m = oreturn x' |>> m'"
   by simp
 
-lemma oreturn_bind_cong_apply [fundef_cong]:
+lemma oreturn_bind_cong_apply[fundef_cong]:
   "\<lbrakk> x = x'; m x' s = m' x' s \<rbrakk> \<Longrightarrow> (oreturn x |>> m) s = (oreturn x' |>> m') s"
   by simp
 
-lemma oreturn_bind_cong2 [fundef_cong]:
+lemma oreturn_bind_cong2[fundef_cong]:
   "\<lbrakk> x = x'; m x' = m' x' \<rbrakk> \<Longrightarrow> (oreturn $ x) |>> m = (oreturn $ x') |>> m'"
   by simp
 
-lemma oreturn_bind_cong2_apply [fundef_cong]:
+lemma oreturn_bind_cong2_apply[fundef_cong]:
   "\<lbrakk> x = x'; m x' s = m' x' s \<rbrakk> \<Longrightarrow> ((oreturn $ x) |>> m) s = ((oreturn $ x') |>> m') s"
   by simp
 
-lemma ocondition_cong [fundef_cong]:
+lemma ocondition_cong[fundef_cong]:
 "\<lbrakk>c = c'; \<And>s. c' s \<Longrightarrow> l s = l' s; \<And>s. \<not>c' s \<Longrightarrow> r s = r' s\<rbrakk>
   \<Longrightarrow> ocondition c l r = ocondition c' l' r'"
   by (auto simp: ocondition_def)
 
 
-text \<open>Decomposition\<close>
+subsection \<open>Decomposition\<close>
 
-lemma ocondition_K_true [simp]:
+lemma ocondition_K_true[simp]:
   "ocondition (\<lambda>_. True) T F = T"
   by (simp add: ocondition_def)
 
-lemma ocondition_K_false [simp]:
+lemma ocondition_K_false[simp]:
   "ocondition (\<lambda>_. False) T F = F"
   by (simp add: ocondition_def)
 
@@ -353,7 +355,7 @@ lemma oreturnE:
   "\<lbrakk>oreturn x s = Some v; v = x \<Longrightarrow> P\<rbrakk> \<Longrightarrow> P"
   by simp
 
-lemma in_ofail [simp]:
+lemma in_ofail[simp]:
   "ofail s \<noteq> Some v"
   by (auto simp: ofail_def K_def)
 
@@ -361,15 +363,15 @@ lemma ofailE:
   "ofail s = Some v \<Longrightarrow> P"
   by simp
 
-lemma in_oassert_eq [simp]:
+lemma in_oassert_eq[simp]:
   "(oassert P s = Some v) = P"
   by (simp add: oassert_def)
 
-lemma oassert_True [simp]:
+lemma oassert_True[simp]:
   "oassert True = oreturn ()"
   by (simp add: oassert_def)
 
-lemma oassert_False [simp]:
+lemma oassert_False[simp]:
   "oassert False = ofail"
   by (simp add: oassert_def)
 
@@ -398,11 +400,10 @@ lemma obind_eqI_full:
      (clarsimp simp: obind_def split: option.splits)
 
 lemma obindE:
-  "\<lbrakk> (f |>> g) s = Some v;
-     \<And>v'. \<lbrakk>f s = Some v'; g v' s = Some v\<rbrakk> \<Longrightarrow> P\<rbrakk> \<Longrightarrow> P"
+  "\<lbrakk> (f |>> g) s = Some v; \<And>v'. \<lbrakk>f s = Some v'; g v' s = Some v\<rbrakk> \<Longrightarrow> P\<rbrakk> \<Longrightarrow> P"
   by (auto simp: in_obind_eq)
 
-lemma in_othrow_eq [simp]:
+lemma in_othrow_eq[simp]:
   "(othrow e s = Some v) = (v = Inl e)"
   by (auto simp: othrow_def K_def)
 
@@ -410,7 +411,7 @@ lemma othrowE:
   "\<lbrakk>othrow e s = Some v; v = Inl e \<Longrightarrow> P\<rbrakk> \<Longrightarrow> P"
   by simp
 
-lemma in_oreturnOk_eq [simp]:
+lemma in_oreturnOk_eq[simp]:
   "(oreturnOk x s = Some v) = (v = Inr x)"
   by (auto simp: oreturnOk_def K_def)
 
@@ -418,8 +419,7 @@ lemma oreturnOkE:
   "\<lbrakk>oreturnOk x s = Some v; v = Inr x \<Longrightarrow> P\<rbrakk> \<Longrightarrow> P"
   by simp
 
-lemmas omonadE [elim!] =
-  obindE oreturnE ofailE othrowE oreturnOkE oassertE
+lemmas omonadE[elim!] = obindE oreturnE ofailE othrowE oreturnOkE oassertE
 
 lemma in_opt_map_Some_eq:
   "((f ||> g) x = Some y) = (\<exists>v. f x = Some v \<and> g v = y)"
@@ -481,10 +481,7 @@ text \<open>
   (without passing through a state)
 \<close>
 
-inductive_set
-  option_while' :: "('a \<Rightarrow> bool) \<Rightarrow> ('a \<Rightarrow> 'a option) \<Rightarrow> 'a option rel"
-  for C B
-where
+inductive_set option_while' :: "('a \<Rightarrow> bool) \<Rightarrow> ('a \<Rightarrow> 'a option) \<Rightarrow> 'a option rel" for C B where
     final: "\<not> C r \<Longrightarrow> (Some r, Some r) \<in> option_while' C B"
   | fail: "\<lbrakk> C r; B r = None \<rbrakk> \<Longrightarrow> (Some r, None) \<in> option_while' C B"
   | step: "\<lbrakk> C r;  B r = Some r'; (Some r', sr'') \<in> option_while' C B \<rbrakk>
@@ -498,10 +495,12 @@ definition
 lemma option_while'_inj:
   assumes "(s,s') \<in> option_while' C B" "(s, s'') \<in> option_while' C B"
   shows "s' = s''"
-  using assms by (induct rule: option_while'.induct) (auto elim: option_while'.cases)
+  using assms
+  by (induct rule: option_while'.induct) (auto elim: option_while'.cases)
 
 lemma option_while'_inj_step:
-  "\<lbrakk> C s; B s = Some s'; (Some s, t) \<in> option_while' C B ; (Some s', t') \<in> option_while' C B \<rbrakk> \<Longrightarrow> t = t'"
+  "\<lbrakk> C s; B s = Some s'; (Some s, t) \<in> option_while' C B ; (Some s', t') \<in> option_while' C B \<rbrakk>
+   \<Longrightarrow> t = t'"
   by (metis option_while'.step option_while'_inj)
 
 lemma option_while'_THE:
@@ -516,9 +515,9 @@ lemma option_while_simps:
   "(Some s, ss') \<in> option_while' C B \<Longrightarrow> option_while C B s = ss'"
   using option_while'_inj_step[of C s B s']
   by (auto simp: option_while_def option_while'_THE
-      intro: option_while'.intros
-      dest: option_while'_inj
-      elim: option_while'.cases)
+           intro: option_while'.intros
+           dest: option_while'_inj
+           elim: option_while'.cases)
 
 lemma option_while_rule:
   assumes "option_while C B s = Some s'"
@@ -582,9 +581,7 @@ qed
 
 section \<open>Lift @{term option_while} to the @{typ "('a,'s) lookup"} monad\<close>
 
-definition
-  owhile :: "('a \<Rightarrow> 's \<Rightarrow> bool) \<Rightarrow> ('a \<Rightarrow> ('s,'a) lookup) \<Rightarrow> 'a \<Rightarrow> ('s,'a) lookup"
-where
+definition owhile :: "('a \<Rightarrow> 's \<Rightarrow> bool) \<Rightarrow> ('a \<Rightarrow> ('s,'a) lookup) \<Rightarrow> 'a \<Rightarrow> ('s,'a) lookup" where
  "owhile c b a \<equiv> \<lambda>s. option_while (\<lambda>a. c a s) (\<lambda>a. b a s) a"
 
 lemma owhile_unroll:
@@ -593,7 +590,7 @@ lemma owhile_unroll:
                  option_while_simps
            split: option.split)
 
-text \<open>rule for terminating loops\<close>
+text \<open>Rule for terminating loops\<close>
 
 lemma owhile_rule:
   assumes "I r s"
